\documentclass[letterpaper]{article}
\input{../../../preamble.tex}
\usepackage[utf8]{inputenc}
\usepackage[english]{babel}
\usepackage{fancyhdr}
\usepackage[hidelinks]{hyperref}

\pagestyle{fancy}
\fancyhf{}
\rhead{Math 170B}
\chead{Monday, April 10, 2023}
\lhead{Lecture 4}
\rfoot{\thepage}

\setlength{\parindent}{0pt}

\begin{document}

\section{Machine (Floating-Point) Numbers (Section 1.3, Continued)}
\begin{mdframed}
    (Example.) Let $x = \frac{2}{3}$. 
    
    \begin{enumerate}[(1)]
        \item What is the binary form of $x$?
        \begin{mdframed}
            The algorithm for finding the binary form of the decimal is as follows: 
            \begin{itemize}
                \item Given $x$, multiply it by 2. If the integer part of the result is 1, set the $i$th bit to 1. Otherwise, set it to 0. 
                \item If the $i$th bit is 1, subtract $x \times 2$ by 1. 
                \item Repeat the above until one of the following occurs: 
                \begin{itemize}
                    \item You hit exactly 1, or 
                    \item You hit 23 bits after the binary point (most likely, you'll see that the bits repeat in some way). 
                \end{itemize}
            \end{itemize}
            \[\begin{aligned}
                \frac{2}{3} \cdot 2 &= \frac{4}{3} \geq 1 &\implies 1 \\ 
                \frac{1}{3} \cdot 2 &= \frac{2}{3} < 0 &\implies 0 \\
                \frac{2}{3} \cdot 2 &= \frac{4}{3} \geq 1 &\implies 1 \\ 
                \frac{1}{3} \cdot 2 &= \frac{2}{3} < 0 &\implies 0 \\
                \frac{2}{3} \cdot 2 &= \frac{4}{3} \geq 1 &\implies 1 \\ 
                \frac{1}{3} \cdot 2 &= \frac{2}{3} < 0 &\implies 0 \\
                \frac{2}{3} \cdot 2 &= \frac{4}{3} \geq 1 &\implies 1 \\ 
                \frac{1}{3} \cdot 2 &= \frac{2}{3} < 0 &\implies 0 \\
                &\vdots
            \end{aligned}\]
            This gives us the binary representation \code{0.1010101010...}. Normalizing this gives us 
            \[(1.01010101010101010101010101010101010\hdots)_2 \times 2^{-1}.\]
        \end{mdframed}
        \item Find $x_\_$ and $x_+$.
        \begin{mdframed}
            Note that $x_\_$ is just what we found in the previous step, but with 23 bits to the right of the binary point,
            \[(1.01010101010101010101010)_2 \times 2^{-1}.\]
            Then, $x_+$ is 
            \[(1.01010101010101010101011)_2 \times 2^{-1}.\] 
        \end{mdframed}
        \item What is $\text{fl}(x)$?
        \begin{mdframed}
            We now consider $x - x_\_$ and $x - x_+$. Here, 
            \begin{itemize}
                \item For $x - x_\_$, 
                \begin{verbatim}
                   1111111111222222222233333333...
          1234567890123456789012345678901234567...

x       1.0101010101010101010101010101010101010 x 10^-1
- x_    1.01010101010101010101010               x 10^-1
        ===============================================
        0.0000000000000000000000010101010101010 x 10^-1\end{verbatim}
                This gives us \[0.101\hdots \times 2^{-24} = \frac{2}{3} \times 2^{-24}.\]
                    
                \item For $x - x_+$, we know this will be negative since $x_+ > x$ (since we're rounding \emph{up}). So, generally, we'll consider $x_+ - x$: 
                \[x_+ - x = (x_+ - x_\_) - (x - x_\_) = \left(2^{-23} \times 2^{-1}\right) - \left(\frac{2}{3} \times 2^{-24}\right) = \frac{1}{3} \times 2^{-24}.\]
                Note that $(x_+ - x_\_) = \left(2^{-23} \times 2^{-1}\right)$ came from 
                \begin{verbatim}
x+      1.01010101010101010101011               x 10^-1
- x_    1.01010101010101010101010               x 10^-1
        ===============================================
        0.00000000000000000000001               x 10^-1\end{verbatim}
                so, we have $2^{-23} \times 10^{-1}$. 
            \end{itemize}
            Notice that $x_{+}$ has the smaller error, so $\text{fl}(x) = x^* = x_{+}$. 
        \end{mdframed}
        \item What is the relative round-off error?  
        \begin{mdframed}
            This is 
            \[\frac{|\text{fl}(x) - x|}{|x|} = \frac{|x_+ - x|}{|x|} = \frac{\frac{1}{3} \times 2^{-24}}{\frac{2}{3}} = 2^{-25}.\]

            Notice that \[\frac{|x^* - x|}{|x|} \leq 2^{-24}.\]
        \end{mdframed}
    \end{enumerate}
    
\end{mdframed}


\end{document}